examples/pseudo_bool/cp_encoding/array/compilation/cpCompileScript.sml
@@ -1,0 +1,14 @@
+(*
+  Compiles the CP encoder + PB checker
+*)
+Theory cpCompile
+Ancestors
+  cpProg
+Libs
+  preamble eval_cake_compile_x64Lib eval_cake_compile_arm8Lib
+
+Theorem cp_compiled =
+  eval_cake_compile_x64 "" main_prog_def "cake_pb_cp.S";
+
+Theorem cp_compiled_arm8 =
+  eval_cake_compile_arm8 "arm8_" main_prog_def "cake_pb_cp_arm8.S";
